src/C_strtoimax/VstProof/AbstractSpecLemmas_new.v
@@ -1,0 +1,831 @@
+Require Import Core.Core Core.Tactics.
+Require Import AbstractSpec.
+Require Import VST.floyd.proofauto.
+Require Import StructTact.StructTactics.
+
+Notation value_until b j l := (value (Z_of_string_loop' (sublist 0 j l) 0 1 b)).
+
+Definition ASN1_INTMAX_MAX := Int64.max_signed.
+Definition upper_boundary := Z.div ASN1_INTMAX_MAX 10.
+Definition last_digit_max := Zmod ASN1_INTMAX_MAX 10.
+Definition last_digit_max_minus := last_digit_max + 1.
+
+(* Lemmas about bounded *)
+Ltac Zbool_to_Prop := try (rewrite Z.leb_le ||
+                           rewrite Z.leb_gt ||
+                           rewrite Z.eqb_eq ||
+                           rewrite Z.eqb_neq).
+
+Lemma is_digit_to_Z : forall c, is_digit c = true -> 0 <= Z_of_char c <= 9.
+Proof.
+  unfold is_digit, Z_of_char.
+  intro.
+  rewrite andb_true_iff in *.
+  repeat Zbool_to_Prop.
+  unfold zero_char, nine_char.
+  nia.
+Qed.
+
+Lemma app_is_digit : forall ls j,
+    0 <= j < Zlength ls ->
+    (forall i : Z, 0 <= i < j -> is_digit (Znth i ls) = true) ->
+    is_digit (Znth j ls) = true ->
+    forall i0 : Z, 0 <= i0 < j + 1 -> is_digit (Znth i0 ls) = true.
+Proof.
+  intros.
+  destruct (zle j i0).
+  - replace i0 with j by nia.
+    eassumption.
+  - eapply H0. nia.
+Qed.
+
+
+Lemma sign_not_digit : forall  i, is_sign i = true -> is_digit i = false.
+Proof.
+  intros.
+  unfold is_sign, is_digit in *.
+  unfold zero_char, plus_char, minus_char, nine_char in *.
+  rewrite andb_false_iff; do 2 rewrite Z.leb_gt.
+  rewrite orb_true_iff in H; do 2 rewrite Z.eqb_eq in H.
+  lia.
+Qed.
+
+Lemma digit_not_sign : forall i, is_digit i = true -> is_sign i = false.
+Proof.
+  intros.
+  unfold is_sign, is_digit in *.
+  unfold zero_char, plus_char, minus_char, nine_char in *.
+  rewrite orb_false_iff; do 2 rewrite Z.eqb_neq.
+  rewrite andb_true_iff in H; do 2 rewrite Z.leb_le in H.
+  lia.
+Qed.
+
+Lemma bounded_bool_to_Prop :
+  forall v, bounded v = true ->  
+       Int64.min_signed <= v <= Int64.max_signed.
+Proof.
+  unfold bounded.
+  intro.
+  rewrite andb_true_iff in *.
+  repeat Zbool_to_Prop.
+  auto.
+Qed.
+
+Lemma bounded'_bool_to_Prop :
+  forall v, bounded' false v = true ->  
+       0<= v <= Int64.max_signed + 1.
+Proof.
+  unfold bounded'.
+  intro.
+  rewrite andb_true_iff in *.
+  repeat Zbool_to_Prop.
+  auto.
+Qed.
+
+Lemma lt_inv64:
+ forall i j,
+   Int64.lt i j = true -> (Int64.signed i < Int64.signed j)%Z.
+Proof.
+intros.
+unfold Int64.lt in H. if_tac in H; inv H. auto.
+Qed.
+
+Lemma lt_false_inv64:
+  forall i j,
+    Int64.lt i j = false -> (Int64.signed i >= Int64.signed j)%Z.
+Proof.
+  intros.
+  unfold Int64.lt in H. if_tac in H; inv H. auto.
+Qed.
+               
+Lemma lt_ub_to_next_bounded'_bool : forall v d,
+    0 <= d <= 9 -> 
+    0 <= v < upper_boundary -> 
+    bounded' false (v*10 + d) = true /\
+    bounded' false (v*10) = true /\
+    bounded' false v = true.
+Proof.
+  unfold upper_boundary.
+  unfold bounded'.
+  intros.
+  repeat rewrite andb_true_iff in *.
+  repeat Zbool_to_Prop.
+  cbn in *.
+  nia.
+Qed.
+
+Lemma lt_ub_to_bounded'_Prop : forall v d,
+    0 <= d <= 9 -> (* is digit *)
+    0 <= v < upper_boundary -> 
+    0 <= v <= Int64.max_signed + 1.
+Proof.
+  unfold upper_boundary.
+  unfold bounded'.
+  intros.
+  cbn in *.
+  nia.
+Qed.
+
+Lemma lt_ub_to_next_bounded'_Prop : forall v d,
+    0 <= d <= 9 -> (* is digit *)
+    0 <= v < upper_boundary -> 
+    0 <= v * 10 + d <= Int64.max_signed + 1 /\
+    0 <= v * 10 <= Int64.max_signed + 1. 
+Proof.
+  unfold upper_boundary.
+  unfold bounded'.
+  intros.
+  cbn in *.
+  nia.
+Qed.
+
+
+Definition upper_boundary_int := (
+         (Int64.divs
+            (Int64.shru (Int64.not (Int64.repr (Int.signed (Int.repr 0))))
+                        (Int64.repr (Int.unsigned (Int.repr 1))))
+            (Int64.repr (Int.signed (Int.repr 10))))).
+
+Lemma lt_ub_to_Z1 : forall v,
+    Int64.min_signed <= v <= Int64.max_signed ->
+    Int64.lt (Int64.repr v) upper_boundary_int = true ->
+    v < upper_boundary.
+  Proof.
+    intros v B Lt.
+    eapply lt_inv64 in Lt.
+  rewrite Int64.signed_repr in *.
+  replace (Int64.signed upper_boundary_int) with upper_boundary
+   in Lt by normalize.
+  all: eassumption.
+Qed.
+
+Lemma upper_boundary_int_repr:
+  upper_boundary_int = 
+  Int64.repr 922337203685477580.
+Proof.
+  reflexivity.
+Qed.
+
+Lemma lt_ub_to_Z2 :  forall v,
+    Int64.min_signed <= v <= Int64.max_signed ->
+    Int64.lt (Int64.repr v) upper_boundary_int = false ->
+    v >= upper_boundary.
+Proof.
+  intros.
+  cbn in *.
+  unfold Int64.lt in H0.
+  destruct zlt in H0; [discriminate|].
+  rewrite upper_boundary_int_repr in g.
+  do 2 rewrite Int64.signed_repr in g; cbn; lia.
+Qed.
+
+Lemma lt_ub_to_Z3 :  forall v,
+    0 <= v <= Int64.max_signed ->
+    Int64.eq (Int64.repr v) upper_boundary_int = true ->
+    v = upper_boundary.
+Proof.
+  intros.
+  unfold Int64.eq in H0.
+  destruct zeq in H0; [|discriminate].
+  rewrite upper_boundary_int_repr in e.
+  replace (Int64.unsigned (Int64.repr 922337203685477580)) 
+    with 922337203685477580 in e by reflexivity.
+  rewrite Int64.unsigned_repr in e; cbn in *; lia.
+Qed.
+
+Definition last_digit_max_minus_int :=
+   (Int64.add
+      (Int64.mods (Int64.shru (Int64.not (Int64.repr 0)) 
+                              (Int64.repr 1)) 
+                  (Int64.repr 10)) 
+      Int64.one).
+
+Lemma last_digit_max_minus_int_repr :
+  last_digit_max_minus_int =
+  Int64.repr (8).
+Proof.
+  reflexivity.
+Qed.
+
+Lemma lt_ub_to_Z4 :  forall i, 
+    0 <= Byte.signed i <= Byte.max_unsigned ->
+    Int64.lt last_digit_max_minus_int 
+             (Int64.repr (Int.signed (Int.sub (Int.repr (Byte.signed i)) 
+                                              (Int.repr 48)))) = true -> 
+    last_digit_max_minus < (Byte.signed i - 48).
+Proof.
+  intros.
+  rewrite last_digit_max_minus_int_repr in H0.
+  unfold Int64.lt, Int.sub in H0; destruct zlt in H0; [|discriminate].
+  replace (Int64.signed (Int64.repr 8)) with 8 in l by reflexivity; 
+    replace (Int.unsigned (Int.repr 48)) with 48 in l by reflexivity.
+  pose proof Byte.signed_range i.
+  rewrite Int.unsigned_repr in l by (cbn in *; lia). 
+  rewrite Int.signed_repr in l by (cbn in *; lia). 
+  rewrite Int64.signed_repr in l by (cbn in *; lia).
+  assumption.
+Qed.
+
+Lemma lt_ub_to_Z5 :  forall v,
+    0 <= v <= Int64.max_signed ->
+    Int64.eq (Int64.repr v) upper_boundary_int = false ->
+    v <> upper_boundary.
+Proof.
+  intros.
+  rewrite upper_boundary_int_repr in H0.
+  unfold Int64.eq in H0; destruct zeq in H0; [discriminate|].
+  do 2 rewrite Int64.unsigned_repr in n; cbn in *; try lia.
+Qed.
+
+Lemma lt_ub_to_Z6 :  forall i,
+    0 <= Byte.signed i <= Byte.max_signed ->
+    Int64.lt last_digit_max_minus_int
+             (Int64.repr (Int.signed (Int.sub (Int.repr (Byte.signed i)) 
+                                              (Int.repr 48)))) = false -> 
+    (Byte.signed i - 48) <= last_digit_max_minus.
+Proof.         
+  intros.
+  rewrite last_digit_max_minus_int_repr in H0.
+  unfold Int64.lt, Int.sub in H0; destruct zlt in H0; [discriminate|].
+  pose proof Byte.signed_range i.
+  do 2 rewrite Int.unsigned_repr in g by (cbn in *; lia).
+  rewrite Int.signed_repr in g by (cbn in *; lia).
+  replace (Int64.signed (Int64.repr 8)) with 8 in g by reflexivity.
+  rewrite Int64.signed_repr in g by (cbn in *; lia).
+  cbn in *; lia.
+Qed.
+
+Lemma eq_ub_not_bounded'_minus : forall v d,
+    0 <= v ->
+    0 <= d <= 9 -> 
+    v = upper_boundary ->
+    d > last_digit_max_minus ->
+    bounded' false (v*10 + d) = false.
+Proof.
+  intros.
+  unfold bounded'; cbn in *.
+  rewrite andb_false_iff; do 2 rewrite Z.leb_gt.
+  lia.
+Qed.
+
+Ltac lt_ub_to_Z H := try (eapply lt_ub_to_Z1 in H ||
+                            eapply lt_ub_to_Z2 in H ||
+                               eapply lt_ub_to_Z3 in H ||
+                                 eapply lt_ub_to_Z4 in H ||
+                                  eapply lt_ub_to_Z5 in H ||
+                                   eapply lt_ub_to_Z6 in H).
+
+(* Lemma lt_ub_bounded'_Prop : forall v d,
+    0 <= d <= 9 ->
+    0 <= v ->
+    Int64.min_signed <= v <= Int64.max_signed ->
+    Int64.lt (Int64.repr v) upper_boundary_int = true ->
+    Int64.min_signed <= v * 10 + d <= Int64.max_signed /\ 
+    Int64.min_signed <= v * 10 <= Int64.max_signed.
+Proof.
+  intros v d D V V' Lt.
+  eapply lt_ub_to_next_bounded'_Prop.
+  eassumption.
+  eapply lt_inv64 in Lt.
+  rewrite Int64.signed_repr in *.
+  replace (Int64.signed upper_boundary_int) with upper_boundary
+   in Lt by normalize.
+  all: nia.
+Qed. *)
+
+Lemma neg_bounded' : forall v, 
+    0 <= v -> 
+    bounded' false v = true -> bounded (-1 * v) = true.
+  Proof.
+    unfold bounded', bounded.
+    cbn.
+    intros v H.
+     repeat rewrite andb_true_iff in *.
+     repeat rewrite Z.leb_le in *;
+    try nia.
+Qed.
+
+                  
+Lemma lt_ub_not_bounded' : forall v d, 
+      0 <= v ->
+      0 <= d <= 9 -> 
+      v > upper_boundary ->
+      bounded' false (v*10 + d) = false.
+Proof.
+  intros.
+  unfold bounded'; cbn in *.
+  rewrite andb_false_iff; do 2 rewrite Z.leb_gt.
+  lia.
+Qed.
+
+Lemma eq_ub_bounded'_minus : forall v d,
+    0 <= v ->
+    0 <= d <= 9 -> 
+    v = upper_boundary ->
+    d <= last_digit_max_minus ->
+    bounded' false (v*10 - d) = true.
+Proof.
+  intros.
+  unfold bounded'; cbn in *.
+  rewrite andb_true_iff; do 2 rewrite Z.leb_le.
+  nia.
+Qed.
+
+Lemma eq_ub_next : forall v d,
+    0 <= v ->
+    0 <= d  -> 
+    v = upper_boundary ->
+    v*10 + d > upper_boundary.
+Proof.
+  intros.
+  cbn in *.
+  lia.
+Qed.
+      
+Lemma eq_ub_bounded'_plus : forall v d, 
+      0 <= v ->
+      0 <= d <= 9 -> 
+      v = upper_boundary ->
+      d <= last_digit_max ->
+      bounded' true (v*10 + d) = true.
+Proof.
+  intros.
+  unfold bounded'; cbn in *.
+  rewrite andb_true_iff; do 2 rewrite Z.leb_le.
+  lia.
+Qed.
+
+Lemma eq_ub_not_bounded'_plus : forall v d, 
+    0 <= v ->
+    0 <= d <= 9 -> 
+    v = upper_boundary ->
+    d > last_digit_max ->
+    bounded' true (v*10 + d) = false.
+Proof.
+  intros.
+  unfold bounded'; cbn in *.
+  rewrite andb_false_iff; do 2 rewrite Z.leb_gt.
+  lia.
+Qed.
+
+
+
+Lemma bounded'_false : forall v w b,
+    bounded' b v = false ->
+    0 <= v <= w ->
+    bounded' b w = false.
+  Proof.
+    destruct b;
+  unfold bounded'; cbn in *;
+  intros;
+  rewrite andb_false_iff in *;
+  repeat rewrite Z.leb_gt in *;
+  nia.
+Qed.
+
+
+Lemma loop_non_neg : forall ls v i, 0 <= v -> 0 <= value (Z_of_string_loop' ls v i false).
+Proof.
+  induction ls.
+  - intuition.
+  - intros.
+    simpl;
+      repeat break_if;
+    simpl; try congruence;
+       eapply is_digit_to_Z in Heqb.
+    eapply IHls.
+    all: nia.
+Qed.
+          
+(* Lemmas about Spec *) 
+
+(* ERROR RANGE *)
+
+Lemma ERROR_RANGE_not_bounded'_loop : forall ls v i b,
+  res (Z_of_string_loop' ls v i b) = ERROR_RANGE ->
+  bounded' b (value (Z_of_string_loop' ls v i b)) = false.
+Proof.
+  induction ls; intros v i b.
+  - discriminate.
+  - cbn.
+ repeat break_match;
+      simpl; try congruence. 
+ eapply IHls; intuition.
+Qed.
+
+
+Lemma Zlength_aux_inc : forall ls i,
+    1 + Zlength_aux i byte ls = Zlength_aux (i + 1) byte ls.
+Proof.
+  induction ls.
+  intros; cbn; lia.
+  cbn.
+  intros.
+  eapply IHls with (i := (Z.succ i)).
+Qed.
+
+Lemma sublist_ERROR_RANGE : forall ls v j i, 
+    0 < j ->
+    res (Z_of_string_loop' (sublist 0 j ls) v i false) = ERROR_RANGE ->
+    res (Z_of_string_loop' ls v i false) = ERROR_RANGE.
+Proof.
+  induction ls; intros v j i.
+  -  
+    unfold sublist; rewrite skipn_nil; rewrite firstn_nil;
+      cbn; discriminate.
+  - 
+    intros J.
+    assert (0 <= j - 1) by lia.
+    replace (sublist 0 j (a :: ls)) with (a :: sublist 0 (j - 1) ls); cbn.
+    repeat break_if;
+      cbn; try congruence.
+    apply Z_le_lt_eq_dec in H; destruct H.
+    eapply IHls with (j := j - 1); assumption.
+    rewrite <-e; cbn; discriminate.
+    unfold sublist; cbn.
+    replace (j - 1 - 0) with (j - 1) by lia; replace (j - 0) with (j) by lia.
+    remember (j - 1) as n; assert (Z.succ n = j) by lia; rewrite <-H0.
+    rewrite Z2Nat.inj_succ by assumption.
+    rewrite firstn_cons; reflexivity.
+Qed.
+
+Lemma ERROR_RANGE_index : forall ls v i j,
+    0 <= j ->
+    j + 1 <= Zlength ls ->
+    res (Z_of_string_loop' ls v i false) = ERROR_RANGE -> 
+    bounded' false (value (Z_of_string_loop' (sublist 0 j ls) v i false)) = true ->
+    bounded' false (value (Z_of_string_loop' (sublist 0 (j + 1) ls) v i false)) = false -> 
+    index (Z_of_string_loop' ls v i false) = j + i.
+Proof.
+  induction ls; intros v i j.
+  -
+    cbn; discriminate.
+  -
+    intros J Z; apply Z_le_lt_eq_dec in J; destruct J.
+    replace (sublist 0 j (a :: ls)) with (a :: sublist 0 (j - 1) ls).
+    replace (sublist 0 (j + 1) (a :: ls)) with (a :: sublist 0 j ls).
+    rewrite Zlength_cons in Z; assert (0 <= j - 1) by lia; 
+      assert (j - 1 + 1 <= Zlength ls) by lia.
+    cbn; repeat break_if; cbn; try congruence.
+    intros.
+    replace (j) with (j - 1 + 1) in H3 by lia.
+    pose proof IHls (v * 10 + Z_of_char a) (i + 1) (j - 1) H H0 H1 H2 H3.
+    replace (j - 1 + (i + 1)) with (j + i) in H4 by lia.
+    assumption.
+    1,2: unfold sublist; cbn.
+    replace (j + 1 - 0) with (Z.succ j) by lia; rewrite Z2Nat.inj_succ by lia; 
+      replace (j - 0) with (j) by lia; rewrite firstn_cons; reflexivity.
+    remember (j - 1) as n; replace (n - 0) with (n) by lia; 
+      replace (j - 0) with (j) by lia; assert (j = Z.succ n) by lia; 
+        rewrite H; rewrite Z2Nat.inj_succ by lia; rewrite firstn_cons; 
+          reflexivity.
+    rewrite <-e; cbn; repeat break_if; cbn; try congruence.
+    reflexivity.
+Qed.
+ 
+(* OK *)
+
+Lemma all_digits_OK_or_ERROR_RANGE_loop : forall ls v i b,
+    (forall i, 0 <= i < Zlength ls -> is_digit (Znth i ls)  = true) ->
+    res (Z_of_string_loop' ls v i b) = OK \/
+    res (Z_of_string_loop' ls v i b) = ERROR_RANGE.
+Proof.
+  - induction ls; intros v0 i0 b DIG.
+    -- autorewrite with sublist in *.
+      auto.
+    -- 
+    cbn.
+    replace (is_digit a) with true.
+    break_if.
+    eapply IHls.
+    (*from V *)
+    (* from DIG *)
+    admit.
+    auto.
+    (* from DIG *)
+    admit.
+Admitted.
+
+(* OK *)
+Lemma OK_index_loop : forall ls b v i,
+  res (Z_of_string_loop' ls v i b) = OK -> 
+  index (Z_of_string_loop' ls v i b) = i + Zlength ls.
+Proof.
+   induction ls; intros b v i.
+  - intuition.
+  - simpl.
+    repeat break_match;
+      autorewrite with sublist;
+      simpl; try congruence.
+    replace (i + Z.succ (Zlength ls)) with
+        ((i+1) + Zlength ls) by nia.
+    specialize (IHls b (v * 10 + Z_of_char a) (i + 1)).
+    intuition.
+Qed.
+
+Lemma OK_index : forall ls,
+    res (Z_of_string' ls) = OK -> 
+    index (Z_of_string' ls) = Zlength ls.
+Proof.
+  destruct ls.
+  - intuition.
+  - simpl.
+    break_if.
+    * repeat break_if;
+      simpl;
+      autorewrite with sublist;
+      try congruence; try nia.
+    * repeat break_if.
+      all: replace (Zlength (i :: i0 :: l))
+                   with (1 + Zlength (i0::l)).
+      all: try eapply OK_index_loop.
+      all: autorewrite with sublist;
+      try nia; simpl; easy.
+Qed.
+
+
+Lemma bounded'_to_OK_loop : forall ls v i b,
+  bounded' b (value (Z_of_string_loop' ls v i b)) = true ->
+  (forall i, 0 <= i < Zlength ls -> is_digit (Znth i ls)  = true) ->
+  res (Z_of_string_loop' ls v i b) = OK.
+Proof.
+  intros.
+  edestruct all_digits_OK_or_ERROR_RANGE_loop with (ls := ls)
+                                                   (v := v)
+  as [Ok | ER];
+    intuition;
+    try eassumption.
+  eapply ERROR_RANGE_not_bounded'_loop in ER.
+  congruence.
+Qed.
+
+Lemma OK_bounded'_loop : forall ls b v i,
+    bounded' b v = true ->
+    res (Z_of_string_loop' ls v i b) = OK ->
+    bounded' b (value (Z_of_string_loop' ls v i b)) = true.
+Proof.
+  induction ls; intros b v i.
+  - simpl; congruence.
+  - cbn.
+    repeat break_match;
+      simpl; try congruence.
+    intros. eapply IHls.
+    all: intuition.
+Qed.
+ 
+Lemma app_char_to_OK_loop : forall ls b i,
+    0 < Zlength ls ->
+    is_sign i = true ->
+    res (Z_of_string_loop' ls 0 1 b) = OK ->
+    res (Z_of_string' (i :: ls)) = OK.
+Proof.
+  intros until i. intros N S Ok.
+  pose proof (sign_not_digit i S).
+  unfold is_sign in S.
+  destruct_orb_hyp.
+  all:
+  simpl;
+    repeat break_if; autorewrite with sublist in *;
+      try nia;
+    try eapply sign_not_digit in S;
+    intuition; try congruence; try eassumption.
+  admit. (* refactor *)
+Admitted.
+
+Lemma is_digit_bounded' : forall b c,
+    is_digit c = true ->
+    bounded' b (Z_of_char c) = true.
+Proof.
+  destruct b.
+  intros.
+  unfold is_digit, bounded', zero_char, nine_char, Z_of_char in *; cbn in *.
+  rewrite andb_true_iff in *.
+  repeat rewrite ->Z.leb_le in *.
+  lia.
+  intros.
+  unfold is_digit, bounded', zero_char, nine_char, Z_of_char in *; cbn in *.
+  rewrite andb_true_iff in *.
+  repeat rewrite ->Z.leb_le in *.
+  lia.
+Qed.
+
+(* EXTRA DATA *)
+             
+Lemma value_next_loop : forall ls v i b r,
+    (res (Z_of_string_loop' ls v i r)) = OK ->
+    is_digit b = true ->
+    value (Z_of_string_loop' (ls ++ [b]) v i r) = 
+    (value (Z_of_string_loop' ls v i r)) * 10 + (Z_of_char b).
+Proof.
+  induction ls; intros.
+  * simpl in *.
+    repeat bool_rewrite.
+    break_if; easy.
+  * simpl in *.
+    break_if.
+    break_if.
+    erewrite IHls.
+    reflexivity.
+    eassumption.
+    all: simpl in *;
+    repeat break_if;
+      try congruence; simpl in *;
+    try congruence.
+Qed.
+
+Lemma EXTRA_DATA_next_loop : forall ls v i b r,
+    (res (Z_of_string_loop' ls v i r)) = OK ->
+    is_digit b = false ->
+    res (Z_of_string_loop' (ls ++ [b]) v i r) = EXTRA_DATA.
+Proof.
+  induction ls; intros.
+  * simpl in *.
+    repeat bool_rewrite.
+    easy.
+  * simpl in *.
+    break_if.
+    break_if.
+    erewrite IHls.
+    reflexivity.
+    eassumption.
+    all: simpl in *;
+    repeat break_if;
+      try congruence; simpl in *;
+    try congruence.
+Qed.
+
+Lemma EXTRA_DATA_index_loop : forall ls v i b r,
+    (res (Z_of_string_loop' ls v i r)) = OK ->
+    is_digit b = false ->
+    index (Z_of_string_loop' (ls ++ [b]) v i r) = Zlength ls + i.
+Proof.
+  induction ls; intros.
+  * simpl in *.
+    repeat bool_rewrite.
+    easy.
+  * simpl in *.
+    break_if.
+    break_if.
+    erewrite IHls.
+    autorewrite with sublist.
+    nia.
+    eassumption.
+    all: simpl in *;
+    repeat break_if;
+      try congruence; simpl in *;
+    try congruence.
+Qed.
+
+Lemma next_value_lt_ub : forall ls j i b,
+     (forall i : Z, 0 <= i < j  ->
+               is_digit (Znth i ls) = true) ->
+     0 < j + 1 <= Zlength ls ->
+     bounded' b (value_until b j ls) = true -> 
+     Znth j ls = i ->
+     is_digit i = true ->
+     (value_until b (j + 1) ls) = (value_until b j ls * 10 + (Z_of_char i)).
+Proof.
+  intros.
+  rewrite sublist_last_1.
+  subst.
+  eapply value_next_loop.
+  eapply bounded'_to_OK_loop.
+  eassumption.
+  admit.
+  eassumption.
+  all: nia.
+Admitted.
+
+Lemma ub_last_digit_error_range : forall j i ls,
+  0 <= j < Zlength ls ->
+  Znth j ls = i ->
+  is_digit i = true ->
+  (forall i0 : Z, 0 <= i0 < j -> is_digit (Znth i0 ls) = true) ->
+  bounded' false (value_until false j ls) = true ->
+  (value_until false j ls > upper_boundary \/
+  (value_until false j ls = upper_boundary /\
+  last_digit_max_minus < (Byte.signed i - 48))) ->
+  (res (Z_of_string_loop' ls 0 1 false)) = ERROR_RANGE.
+Proof.
+  intros.
+  inversion H4.
+  - 
+  inversion H3.
+  eapply bounded'_bool_to_Prop in H3.
+  assert (bounded' false (value_until false (j + 1) ls) = false) as Bound.
+  { erewrite next_value_lt_ub.
+    eapply lt_ub_not_bounded'.
+    eapply loop_non_neg; nia.
+    eapply is_digit_to_Z; eassumption.
+    all: unfold value_until, Z_of_char in *;
+      try eassumption; try nia. }
+
+  assert (res (Z_of_string_loop' ls 0 1 false) = ERROR_RANGE) as Result_loop.
+  { edestruct all_digits_OK_or_ERROR_RANGE_loop
+      with (ls := sublist 0 (j + 1) ls) (v := 0) (i := 1) (b := false) as [Ok | Er].
+    autorewrite with sublist.
+    admit.
+    inversion Ok.
+    eapply OK_bounded'_loop in Ok.
+    congruence.
+    admit.
+    eapply sublist_ERROR_RANGE in Er.
+    rewrite Er.
+    reflexivity.
+    nia.
+  }
+  eassumption.
+  - 
+    inversion H3.
+  eapply bounded'_bool_to_Prop in H3.
+  assert (bounded' false (value_until false (j + 1) ls) = false) as Bound.
+  { erewrite next_value_lt_ub.
+    eapply eq_ub_not_bounded'_minus.
+    eapply loop_non_neg; nia.
+    eapply is_digit_to_Z; eassumption.
+    all: unfold value_until, Z_of_char in *;
+      try eassumption; try nia. }
+
+  assert (res (Z_of_string_loop' ls 0 1 false) = ERROR_RANGE) as Result_loop.
+
+  { edestruct all_digits_OK_or_ERROR_RANGE_loop
+      with (ls := sublist 0 (j + 1) ls) (v := 0) (i := 1) (b := false)  as [Ok | Er].
+    autorewrite with sublist.
+    admit.
+    inversion Ok.
+    eapply OK_bounded'_loop in Ok.
+    congruence.
+    admit.
+    eapply sublist_ERROR_RANGE in Er.
+    rewrite Er.
+    reflexivity.    
+    nia.
+  }
+  eassumption.
+Admitted.
+
+(* EXTRA DATA *)
+
+Lemma EXTRA_DATA_or_ERROR_RANGE_result :
+  forall ls v k j i b, 
+    0 <= j < Zlength ls ->
+    Znth j ls = i -> 
+    is_digit i = false -> 
+    res (Z_of_string_loop' ls v k b) = EXTRA_DATA
+    \/ res (Z_of_string_loop' ls v k b) = ERROR_RANGE.
+  induction ls; intros v k j i b N Dig Bound.
+  - autorewrite with sublist in *.
+    nia.
+  - simpl.
+    repeat break_if.
+    assert (0 <= Zlength ls).
+    eapply Zlength_nonneg.
+    assert (0 < j) as ZZ.
+    destruct (zle 0 (j -1)).
+    nia.
+    assert (j = 0) as Z by nia.
+    rewrite Z in Dig.
+    erewrite Znth_0_cons in Dig.
+    subst.
+    congruence.
+    eapply IHls with (j := j - 1) (i := i).  
+    autorewrite with sublist in *.
+    auto with zarith.
+    rewrite <- Dig.
+    erewrite Znth_pos_cons; auto.
+    eassumption.
+    all: intuition. 
+Qed.
+
+Lemma EXTRA_DATA_value_loop : forall ls v i b r,
+    (res (Z_of_string_loop' ls v i r)) = OK ->
+    is_digit b = false ->
+    value (Z_of_string_loop' (app ls [b]) v i r) =  
+    value (Z_of_string_loop' ls v i r).
+Proof.
+  induction ls; intros.
+  * simpl in *.
+    repeat bool_rewrite.
+    easy.
+  * simpl in *.
+    break_if.
+    break_if.
+    erewrite IHls.
+    autorewrite with sublist.
+    nia.
+    eassumption.
+    all: simpl in *;
+      repeat break_if;
+      try congruence; simpl in *;
+        try congruence.
+Qed.
+
+Lemma sublist_EXTRA_DATA : forall ls v j i m vl b, 
+    res (Z_of_string_loop' (sublist 0 j ls) v i b) = EXTRA_DATA ->
+    value (Z_of_string_loop' (sublist 0 j ls) v i b) = vl ->
+    index (Z_of_string_loop' (sublist 0 j ls) v i b) = m ->
+
+    res (Z_of_string_loop' ls v i b) = EXTRA_DATA /\
+    index (Z_of_string_loop' ls v i b) = m /\
+    value (Z_of_string_loop' ls v i b) = vl.
+Admitted.
