src/C_strtoimax/VstProof/Proof_new.v
@@ -1,0 +1,1302 @@
+Require Import Core.Tactics Core.PtrLemmas.
+Require Import StructTact.StructTactics Psatz.
+Require Import SepLemmas.
+Require Import AbstractSpec AbstractSpecLemmas_new.
+Require Import VST.floyd.proofauto Psatz.
+Require Import Clight.INTEGER.
+Arguments valid_pointer p : simpl never.
+
+Ltac test_order_ptrs_tac p1 p2 :=
+          unfold test_order_ptrs; simpl;
+          destruct peq; [simpl|contradiction];
+          apply andp_right;
+          [try (apply derives_trans with (Q := valid_pointer p1);
+          entailer!;
+          apply valid_pointer_weak) | try (
+          apply derives_trans with (Q := valid_pointer p2);
+          entailer!;
+          apply valid_pointer_weak)]. 
+
+Definition Vprog : varspecs. mk_varspecs prog. Defined.
+Instance CompSpecs : compspecs. make_compspecs prog. Defined.
+
+Require Import AbstractSpec.
+
+Definition asn_strtoimax_lim_vst_spec : ident * funspec :=
+  DECLARE _asn_strtoimax_lim
+    (* WITH: binds variables in Pre- and Postconditions *)
+    WITH (* start of the string str *)
+         str_b : block, str_ofs : ptrofs,
+         (* end of the string *end *)
+         end'_b : block, end'_ofs : ptrofs,
+         (* stores address of the end of the string end *)
+         end_b : block, end_ofs : ptrofs,
+         (* stores result intp *)
+         intp_b : block, intp_ofs : ptrofs,
+         (* permission shares, cf. Verifiable C book (p.73) *)
+         sh_str : share, sh_end : share, sh_intp : share,
+         (* input string *)
+         ls : list byte,
+         (* ls of intp *)
+         v : val
+    (* Preconditions *)
+    (* Type declaration for parameters of the function *)
+    PRE [ _str OF (tptr tschar),
+          _end OF (tptr (tptr tschar)),
+          _intp OF (tptr tlong) ]
+    (* PROP: Propositions (of type Prop) that should hold
+       before executing the function. ; is conjuction *)
+    
+    PROP ( (* Permissions for memory access *)
+          readable_share sh_str;  (* str points to readable memory *)
+          writable_share sh_end;  (* end points to writable memory *)
+          writable_share sh_intp; (* intp points to writable memory *)
+
+          (* str and end' should point to the same object, 
+           otherwise incomparable by C standard *)
+          str_b = end'_b;
+
+          (* length of ls = distance between str and end' *)
+          Zlength ls =
+          Z.max 0 (Ptrofs.unsigned end'_ofs - Ptrofs.unsigned str_ofs);
+
+         (* No pointer overflow occurs *)
+         Ptrofs.unsigned str_ofs + Zlength ls < Ptrofs.modulus        
+                
+      )
+      (* LOCAL: connects C light prameter identifiers and declared variables *)
+      LOCAL (temp _str (Vptr str_b str_ofs);
+             temp _end (Vptr end_b end_ofs); 
+             temp _intp (Vptr intp_b intp_ofs))
+      (* SEP: Propositions about memory (of type mem -> Prop (mpred)) that 
+         should hold before executing the function. 
+         ; (and * ) is separating conjunction, && is ordinary conjuction *)
+                     
+      SEP ((* str and end' are comparable, i.e. point within the same object *)
+        valid_pointer (Vptr end'_b (Ptrofs.add str_ofs (Ptrofs.repr
+                                                          (Zlength ls)))) ;
+           valid_pointer (Vptr end'_b end'_ofs) ;
+           valid_pointer (Vptr str_b str_ofs) ;
+           (* str points to ls with readable permission *)
+           data_at sh_str (tarray tschar (Zlength ls)) 
+                   (map Vbyte ls) (Vptr str_b str_ofs) ; 
+           (* end points to end' with writable permission *)
+           data_at sh_end (tptr tschar) (Vptr end'_b end'_ofs) 
+                   (Vptr end_b end_ofs);
+           (* intp points to some value v  *)
+           data_at sh_intp (tlong) v (Vptr intp_b intp_ofs))     
+    (* Postconditions *)
+    (* Type declaration for return value of the function *)
+    POST [tint]
+      (* No new propositions hold after executing the function *)
+      PROP()
+      (* Return value of the function corresponds to the result 
+         of abstract spec on ls *)
+      LOCAL (temp ret_temp (Vint (asn_strtox_result_e_to_int 
+                                   (res 
+                                      (Z_of_string' ls)))))
+      (* Propositions about memory that hold after executing the function *)
+      SEP( (* this part didn't change after execution *) 
+           
+           valid_pointer (Vptr end'_b end'_ofs) ;
+           valid_pointer (Vptr str_b str_ofs) ;
+           data_at sh_str (tarray tschar (Zlength ls)) 
+                   (map Vbyte ls) (Vptr str_b str_ofs) ;
+           let r := res (Z_of_string' ls) in
+            (* in 3 cases intp stays unchanged,
+              otherwise store the end value of Z_of_string' *)
+            match r with 
+              | ERROR_RANGE 
+              | ERROR_INVAL 
+              | EXPECT_MORE => 
+                data_at sh_intp (tlong) v (Vptr intp_b intp_ofs)
+              | _ => data_at sh_intp (tlong) 
+                         (Vlong (Int64.repr (value (Z_of_string' ls))))
+                         (Vptr intp_b intp_ofs) 
+            end ;
+           (* if str >= end, end doesn't change, 
+              otherwise store the address of the last char read 
+              (before going out of range, reading extra data 
+              or successfully terminating) *)
+            let i := index (Z_of_string' ls) in
+            if (Ptrofs.unsigned str_ofs <? Ptrofs.unsigned end'_ofs)
+            then data_at sh_end (tptr tschar) 
+                         (Vptr str_b (Ptrofs.add str_ofs (Ptrofs.repr i))) 
+                         (Vptr end_b end_ofs)
+            else data_at sh_end (tptr tschar) (Vptr end'_b end'_ofs) 
+                         (Vptr end_b end_ofs)).
+
+
+Definition Gprog := ltac:(with_library prog [asn_strtoimax_lim_vst_spec]).
+
+Lemma body_asn_strtoimax_lim : semax_body Vprog Gprog f_asn_strtoimax_lim
+                                          asn_strtoimax_lim_vst_spec.
+Proof.
+  start_function.
+  pose (upper_boundary := (
+         (Int64.divs
+            (Int64.shru (Int64.not (Int64.repr (Int.signed (Int.repr 0))))
+                        (Int64.repr (Int.unsigned (Int.repr 1))))
+            (Int64.repr (Int.signed (Int.repr 10)))))).
+  pose (last_digit_max := ((Int64.mods
+                                    (Int64.shru
+                                       (Int64.not (Int64.repr 0))
+                                       (Int64.repr 1))
+                                    (Int64.repr 10)))).
+  rename H into EQB.
+  rename H0 into LEN.
+  all: repeat forward; try entailer!.         
+  1-2: break_and; inversion H7.
+  destruct Z.ltb eqn:IFCON.
+  - (* str < end' = true *)
+    all: Intros.
+    forward_if; apply Z.ltb_lt in IFCON.
+    + (* Valid pointer proof *)
+     test_order_ptrs_tac (Vptr end'_b str_ofs) (Vptr end'_b end'_ofs).
+    + (*  srt >= end' from forward_if : contradiction *)
+      forward.
+      apply typed_true_ptr_ge in H.
+      rewrite Z.geb_le in H; Lia.lia.
+    + (*  str < end' = true from forward_if, go further in the branch *)
+      rewrite EQB in H; apply typed_false_ptr_ge in H.
+      rewrite Z.gtb_lt in H.
+      assert (0 < Ptrofs.unsigned end'_ofs - Ptrofs.unsigned str_ofs)
+        by Lia.lia.
+      destruct ls.
+      replace (Zlength []) with (0) in LEN by reflexivity.
+      Lia.lia.
+      erewrite split_non_empty_list with (ls' := ls) (i := i) (ofs := str_ofs).
+      autorewrite with sublist in LEN.
+      assert (Zlength ls = (Ptrofs.unsigned end'_ofs - 
+                                 Ptrofs.unsigned str_ofs) - 1) as LS_len by nia.
+      Intros.
+      repeat forward.
+           pose (sep_precondition :=
+              SEP  (
+                   valid_pointer (Vptr end'_b end'_ofs);
+                   valid_pointer (Vptr str_b str_ofs);
+                   data_at sh_str tschar (Vbyte i) (Vptr str_b str_ofs);
+                   data_at sh_str (tarray tschar (Zlength ls)) (map Vbyte ls)
+                           (Vptr str_b (Ptrofs.add str_ofs Ptrofs.one));
+                   data_at sh_end (tptr tschar) (Vptr end'_b end'_ofs)
+                           (Vptr end_b end_ofs);
+                   data_at sh_intp tlong v (Vptr intp_b intp_ofs))).
+      forward_if (
+          if Byte.signed i =? 45
+          then PROP(1 < Zlength ls)
+               LOCAL(temp _sign (Vint (Int.repr (-1)));
+                     temp _str (Vptr end'_b
+                                     (Ptrofs.add str_ofs (Ptrofs.repr 1)));
+                     temp _end (Vptr end_b end_ofs); 
+                     temp _intp (Vptr intp_b intp_ofs);
+                     temp _last_digit_max
+                          (Vlong (Int64.add last_digit_max Int64.one));
+                     temp _upper_boundary (Vlong upper_boundary))
+               sep_precondition
+          else if Byte.signed i =? 43
+               then PROP(1 < Zlength ls)
+                    LOCAL(temp _str (Vptr end'_b 
+                                          (Ptrofs.add str_ofs (Ptrofs.repr 1)));
+                         temp _end (Vptr end_b end_ofs); 
+                     temp _intp (Vptr intp_b intp_ofs))
+                    sep_precondition
+               else !!(Byte.signed i =? 43 = false /\
+                       Byte.signed i =? 45 = false)).
+      * (* if *str = '-' = Int.repr 45 *)
+        admit.
+      * (* if *str = '+' *)
+        admit.
+      * (* default case *) 
+        admit.
+      * (* Loop *)
+        repeat break_if;
+          unfold sep_precondition.
+        ** forward.
+           remember (Ptrofs.add str_ofs Ptrofs.one) as str_ofs'.
+           remember (Int64.unsigned upper_boundary) as ub.
+           remember (i :: ls) as ls'.
+           forward_loop (
+               EX j : Z, EX vl : Z, 
+                 let i' := Ptrofs.add str_ofs (Ptrofs.repr (j + 1)) in
+                 PROP(0 <= j <= Zlength ls;
+                      Ptrofs.unsigned str_ofs + j + 1 < Ptrofs.modulus;
+                      forall i : Z, 0 <= i < j -> is_digit (Znth i ls) = true;
+                        bounded' false (value_until false j ls) = true)
+                 LOCAL(temp _end (Vptr end_b end_ofs); 
+                       temp _intp (Vptr intp_b intp_ofs);
+                       temp _str (Vptr end'_b i');
+                       temp _value (Vlong (Int64.repr (value_until false  j ls))) ;
+                       temp _sign (Vint (Int.repr (-1)));
+                       temp _upper_boundary (Vlong upper_boundary);
+                       temp _last_digit_max
+                            (Vlong (Int64.add last_digit_max Int64.one)))
+                 SEP(
+                   valid_pointer (Vptr end'_b str_ofs) ;
+                   valid_pointer (Vptr end'_b end'_ofs) ;
+                   (* str |-> i *)                  
+                   data_at sh_str tschar (Vbyte i)
+                           (Vptr end'_b str_ofs);                  
+                   (* str + 1 |-> sublist 1 (j + 1) ls *)
+                   data_at sh_str (tarray tschar j)
+                           (map Vbyte (sublist 0 j ls))
+                            (Vptr end'_b str_ofs');                   
+                   (* str + j + 1 |-> sublist (j + 1) |ls'| ls'  *)
+                   data_at sh_str (tarray tschar (Zlength ls - j))
+                           (map Vbyte (sublist j (Zlength ls) ls))
+                           (Vptr end'_b i') ; 
+                   data_at sh_end (tptr tschar) (Vptr end'_b end'_ofs)
+                           (Vptr end_b end_ofs) ;
+                   data_at sh_intp tlong v (Vptr intp_b intp_ofs)))
+               
+           break: ( EX j : Z,
+                   PROP(0 <= j <= Zlength ls;
+                       forall i, 0 <= i < Zlength ls -> 
+                            is_digit (Znth i ls) = true;
+                        bounded' false (value (Z_of_string_loop' ls 0 1 false)) = true)
+                   LOCAL(
+                     temp _value 
+                          (Vlong (Int64.repr 
+                                    (if Ptrofs.unsigned str_ofs + j + 1 >=? 
+                                        Ptrofs.unsigned end'_ofs  
+                                    then value (Z_of_string_loop' ls 0 1 false)
+                                    else -1 * (value (Z_of_string_loop' ls 0 1 false)))));
+                      temp _sign 
+                          (Vint (Int.repr 
+                                    (if Ptrofs.unsigned str_ofs + j + 1 >=? 
+                                        Ptrofs.unsigned end'_ofs
+                                    then -1
+                                    else 1)));
+
+                   temp _end (Vptr end_b end_ofs); 
+                   temp _intp (Vptr intp_b intp_ofs);
+                   temp _str (Vptr end'_b 
+                              (Ptrofs.add str_ofs 
+                                          (Ptrofs.repr (Zlength ls + 1)))))
+
+                   SEP(
+                     
+                    valid_pointer (Vptr end'_b end'_ofs);
+                    valid_pointer (Vptr end'_b str_ofs);
+                    data_at sh_str (tarray tschar (Zlength ls + 1)) 
+                            (map Vbyte (i::ls)) (Vptr end'_b str_ofs); 
+                    data_at sh_end (tptr tschar) (Vptr end'_b end'_ofs) 
+                            (Vptr end_b end_ofs);
+                    data_at sh_intp (tlong) v (Vptr intp_b intp_ofs))).
+           (* BREAK IMPLIES THE REST OF THE FUNCTION *)
+           3: 
+             { Intro j.
+               forward.
+               forward.
+               entailer!.
+               unfold bounded' in *.
+               rewrite andb_true_iff in *.
+               repeat rewrite Z.leb_le in *.
+               break_if.
+               1-2: repeat rewrite Int64.signed_repr;
+               repeat rewrite Int.signed_repr;
+               rep_omega_setup;
+               assert (0 <= value (Z_of_string_loop' ls 0 1 false)) by 
+               (eapply loop_non_neg; nia);
+               try nia;
+               try rep_omega.
+               admit.
+               forward.
+               assert (res (Z_of_string' (i :: ls)) = OK) as OK.
+               { erewrite app_char_to_OK_loop. 
+                 reflexivity.
+                 nia.
+                 unfold is_sign, minus_char.
+                 bool_rewrite.
+                 intuition.               
+                 eapply bounded'_to_OK_loop; try (nia || eassumption). }
+                assert (index (Z_of_string' (i :: ls)) = Zlength (i::ls))
+                 as I.
+               eapply OK_index.
+               eassumption.
+               assert (((-1) * value (Z_of_string_loop' ls 0 1 false))%Z = 
+                       (value (Z_of_string' (i :: ls)))) as V.
+               { simpl.
+                 unfold is_sign, minus_char.
+                 bool_rewrite.
+                 break_match.
+                 autorewrite with sublist in *.
+                 nia.
+                 replace (Byte.signed i =? plus_char) 
+                         with false.
+                 reflexivity.
+                 symmetry.
+                 Zbool_to_Prop.
+                 rewrite Z.eqb_eq in *.
+                 unfold plus_char.
+                 nia.
+               }
+                 erewrite OK, I, V.  
+                 all: 
+               break_if; entailer;
+                    try erewrite V;
+                   autorewrite with sublist; entailer!. }
+           ***
+             Exists 0 0.
+             entailer!.
+             { intros. nia.
+                }
+             autorewrite with sublist.
+             erewrite data_at_zero_array_eq.
+             entailer!.
+             all: try (erewrite sublist_1_cons || autorewrite with sublist);
+               autorewrite with sublist; (reflexivity || auto with zarith || auto).
+           ***
+             assert (is_sign i = true) as SGN by admit.
+             assert (Byte.signed i =? minus_char = true) as MCH by admit.
+             assert (Byte.signed i =? plus_char = false) as PCH by admit.
+             Intros j vl.
+             assert (0 <= value_until false j ls) as NN by (eapply loop_non_neg; nia).
+             forward.
+             forward_if.
+           3:
+             { (* BREAK: str + j + 1 >= end *)
+             forward.
+             rewrite_comparison.
+             replace (Ptrofs.unsigned (Ptrofs.add str_ofs (Ptrofs.repr (j + 1))))
+                     with (Ptrofs.unsigned str_ofs + j + 1) in *
+               by (autorewrite with norm;
+                   ptrofs_compute_add_mul;
+                   rep_omega_setup;
+                   nia).
+             (* post-if implies break condition *)
+             { Exists j.
+               replace (Ptrofs.unsigned str_ofs + j + 1 >=?
+                                                        Ptrofs.unsigned end'_ofs)
+                       with true.
+               replace j with (Zlength ls) in * by nia.
+               replace (Zlength ls + 1) with
+                   (Zlength (i::ls)) by (autorewrite with sublist; nia).
+               erewrite  split_data_at_sublist_tschar with 
+                   (ls := i :: ls) (j := 1).
+               autorewrite with sublist.
+               replace (Z.succ (Zlength ls) - 1)
+                           with (Zlength ls) by nia.     
+               unfold value_until in *.
+               autorewrite with  sublist in *.
+               entailer!.
+               erewrite data_at_zero_array_eq.
+               entailer!.
+               replace (sublist 1 (Z.succ (Zlength ls)) (i :: ls)) with
+                   ls.
+               erewrite data_at_singleton_array_eq.
+               entailer!.
+               auto.
+               replace (Z.succ (Zlength ls) - 1)
+                 with (Zlength ls) by nia.
+               all: try (erewrite sublist_1_cons || autorewrite with sublist);
+                 autorewrite with sublist; (reflexivity || auto with zarith || auto).
+               symmetry.
+               erewrite Z.geb_le.
+               nia. }
+             }
+              (* pointer comparison *)
+             { unfold test_order_ptrs; simpl.
+               destruct peq; [simpl|contradiction].
+               apply andp_right.
+               destruct (Z_lt_le_dec j (Zlength ls)).
+               * apply derives_trans with (Q := valid_pointer
+                                        (Vptr end'_b (Ptrofs.add str_ofs 
+                                                        (Ptrofs.repr (j + 1))))).
+                 entailer!.
+                 apply valid_pointer_weak.
+               * apply derives_trans with (Q := valid_pointer (Vptr end'_b end'_ofs)).
+                 entailer!.
+                 replace end'_ofs with (Ptrofs.add str_ofs (Ptrofs.repr (j + 1))).
+                 apply valid_pointer_weak.
+                 { autorewrite with sublist in LEN.
+                   replace (Zlength ls) with j in LEN by nia.
+                   assert (Ptrofs.unsigned str_ofs + 1 + j = Ptrofs.unsigned end'_ofs) by nia.
+                   ptrofs_compute_add_mul.
+                   replace end'_ofs with (Ptrofs.repr (Ptrofs.unsigned end'_ofs))
+                     by auto with ints.
+                   f_equal.
+                   all: rep_omega_setup; try nia. }
+               * apply derives_trans with (Q := valid_pointer (Vptr end'_b end'_ofs)).
+                 entailer!.
+                 apply valid_pointer_weak.
+             }
+             (* str + j + 1 <  end *)
+           { rewrite_comparison.
+             replace (Ptrofs.unsigned (Ptrofs.add str_ofs (Ptrofs.repr (j + 1)))) 
+                           with (Ptrofs.unsigned str_ofs + (j + 1)) in * by
+                 (ptrofs_compute_add_mul;
+                  rep_omega_setup;
+                  nia).
+             assert (j < Zlength ls) as jLS by nia.
+             assert (0 < Zlength (sublist j (Zlength ls) ls)) by
+                  (autorewrite with sublist; nia).
+             (* reading a char i0 *)
+             edestruct sublist_first with (j := j) (ls := ls) as [i0 Sub];
+               try nia.
+             econstructor.
+             instantiate (1 := 0).
+             cbv; easy.
+              assert (Znth j ls = i0) as ZN.
+             { replace (i0 :: sublist (j + 1) (Zlength ls) ls)
+                       with (app [i0] (sublist (j + 1) (Zlength ls) ls))
+                            in Sub.
+               erewrite <- sublist_rejoin' 
+                        with (mid := j + 1)
+                             (mid' := j + 1) in Sub.
+               eapply app_inv_tail in Sub.
+               erewrite  sublist_len_1 in Sub.
+               inversion Sub.
+               all: auto.
+               all: try nia. }                   
+             assert (data_at sh_str (tarray tschar (Zlength ls - j))
+                             (map Vbyte (sublist j (Zlength ls) ls))
+                             (Vptr end'_b (Ptrofs.add str_ofs (Ptrofs.repr (j + 1)))) = 
+                             data_at sh_str tschar (Vbyte i0)
+                                     (Vptr end'_b (Ptrofs.add str_ofs (Ptrofs.repr (j + 1)))) *
+                             data_at sh_str (tarray tschar
+                                                    (Zlength (sublist (j + 1) (Zlength ls) ls)))
+                                     (map Vbyte (sublist (j + 1) (Zlength ls) ls))
+                                     (Vptr end'_b (Ptrofs.add (Ptrofs.add str_ofs
+                                            (Ptrofs.repr (j + 1))) Ptrofs.one))) as DATA_AT1.
+             { erewrite Sub.
+               replace (Zlength ls - j) with
+                   (Zlength ((i0::(sublist (j + 1) (Zlength ls) ls)))).               
+            
+               erewrite split_non_empty_list with 
+                   (i := i0) 
+                   (ls' := (sublist (j + 1) (Zlength ls) ls))
+                   (ofs := (Ptrofs.add str_ofs (Ptrofs.repr (j + 1)))); 
+                 try reflexivity.
+               1-2: autorewrite with sublist;
+                 ptrofs_compute_add_mul;
+                 rep_omega_setup; try nia. }   
+              assert (data_at sh_str (tarray tschar (Zlength ls)) (map Vbyte ls)
+                             (Vptr end'_b (Ptrofs.add str_ofs Ptrofs.one)) =
+                     data_at sh_str (tarray tschar j) (map Vbyte (sublist 0 j ls))
+                             (Vptr end'_b (Ptrofs.add str_ofs Ptrofs.one)) *
+                     data_at sh_str (tarray tschar (Zlength ls - j))
+                             (map Vbyte (sublist j (Zlength ls) ls))
+          (Vptr end'_b (Ptrofs.add str_ofs (Ptrofs.repr (j + 1))))) as DATA_AT2.
+             { replace (Ptrofs.add str_ofs (Ptrofs.repr (j + 1))) with
+                 (Ptrofs.add (Ptrofs.add str_ofs Ptrofs.one) (Ptrofs.repr j)).
+               erewrite <- split_data_at_sublist_tschar; try
+               reflexivity. 
+               all: 
+                ptrofs_compute_add_mul;
+                replace (Ptrofs.unsigned Ptrofs.one)
+                           with 1 by auto with ptrofs;
+                rep_omega_setup; try (nia || f_equal); try nia. }
+
+             assert (
+               data_at sh_str (tarray tschar (Zlength ls)) (map Vbyte ls)
+                             (Vptr end'_b (Ptrofs.add str_ofs Ptrofs.one)) =
+               data_at sh_str (tarray tschar (j + 1)) (map Vbyte (sublist 0 (j + 1) ls))
+                             (Vptr end'_b (Ptrofs.add str_ofs Ptrofs.one)) *
+                     data_at sh_str (tarray tschar (Zlength ls - (j + 1)))
+                             (map Vbyte (sublist (j + 1) (Zlength ls) ls))
+                             (Vptr end'_b (Ptrofs.add str_ofs (Ptrofs.repr (j + 1 + 1)))))
+             as DATA_AT3.
+             { replace (Ptrofs.add str_ofs (Ptrofs.repr (j + 1 + 1))) 
+                 with (Ptrofs.add (Ptrofs.add str_ofs Ptrofs.one) (Ptrofs.repr (j + 1))).
+               erewrite <- split_data_at_sublist_tschar.
+               reflexivity.
+               all: 
+                 ptrofs_compute_add_mul;
+                 replace (Ptrofs.unsigned Ptrofs.one)
+                   with 1 by auto with ptrofs;
+                 rep_omega_setup; try (nia || f_equal); try nia. }
+             erewrite DATA_AT1.
+             Intros.
+             forward.
+             forward_if (temp _t'2
+                              (if 48 <=? Byte.signed i0 
+                               then (Val.of_bool (Byte.signed i0 <=? 57))
+                               else  Vfalse)).
+             forward.
+             forward.
+             entailer!.
+             { erewrite Z.ge_le_iff in *.
+               erewrite <- Z.leb_le in *.
+               break_if.
+               replace (negb (Int.lt (Int.repr 57) (Int.repr (Byte.signed (Znth j ls)))))
+                 with (Byte.signed (Znth j ls) <=? 57).
+               destruct (Byte.signed (Znth j ls) <=? 57); easy.
+               eapply Zge_bool_Intge.
+               easy. }
+             forward.
+             entailer!.
+             { break_if.
+               try rewrite <- Zle_is_le_bool in *.
+               nia.
+               reflexivity. }
+             forward_if.
+             eapply typed_true_to_digit in H9.
+             forward.
+             forward.
+             forward_if.
+            (* Case:  vl < ub *)
+           { pose proof (bounded'_bool_to_Prop _ H6).
+             pose proof (is_digit_to_Z i0 H9).
+              lt_ub_to_Z  H10; try nia.
+             forward.
+             entailer!.
+             { repeat rewrite Int64.signed_repr.
+                eapply lt_ub_to_next_bounded'_Prop.
+                 try eassumption; try nia.
+                 all: try nia.
+                  eapply lt_ub_to_next_bounded'_Prop.
+                 try eassumption; try nia.
+                 all: try nia. }
+             forward.
+             (* show that loop invariant holds after normal  loop body execution *)
+             Exists (j + 1) (value_until false (j + 1) ls).
+             entailer!.
+             erewrite next_value_lt_ub with (i := Znth j ls).
+             repeat split; try nia.
+             eapply app_is_digit; try nia; try eassumption.
+             apply lt_ub_to_next_bounded'_bool.
+             all: try eassumption; try nia; auto.
+             entailer!.
+             erewrite sepcon_assoc.
+             erewrite <- DATA_AT1.
+             rewrite <- DATA_AT2, <- DATA_AT3.
+             entailer!.
+           }
+             forward_if.
+           (* vl == ub *)
+           { forward_if.
+             (* d <= last_digit_max *)
+             { forward_if 
+                 (PROP ( )
+     LOCAL (
+       temp _value (Vlong (Int64.repr 
+(- value (Z_of_string_loop' (sublist 0 j ls) 0 1) * 10 - (Byte.signed i0 - 48))));
+       temp _sign (Vint (Int.repr 1));
+
+       temp _d (Vint (Int.sub (Int.repr (Byte.signed i0)) (Int.repr 48)));
+       temp _t'6 (Vbyte i0);
+       temp _t'2 (if 48 <=? Byte.signed i0 
+                  then Val.of_bool (Byte.signed i0 <=? 57) 
+                  else Vfalse);
+       temp _t'7 (Vbyte i0); temp _t'9 (Vptr end'_b end'_ofs); 
+       temp _end (Vptr end_b end_ofs);
+       temp _intp (Vptr intp_b intp_ofs);
+       temp _str (Vptr end'_b (Ptrofs.add str_ofs (Ptrofs.repr (j + 1))));
+       
+       temp _upper_boundary (Vlong upper_boundary);
+       temp _last_digit_max (Vlong (Int64.add last_digit_max Int64.one)))
+     SEP (
+       valid_pointer (Vptr end'_b str_ofs);
+       valid_pointer (Vptr end'_b end'_ofs);
+       data_at sh_str tschar (Vbyte i) (Vptr end'_b str_ofs);
+       data_at sh_str (tarray tschar j) (map Vbyte (sublist 0 j ls)) (Vptr end'_b str_ofs');
+       data_at sh_str tschar (Vbyte i0) (Vptr end'_b (Ptrofs.add str_ofs (Ptrofs.repr (j + 1))));
+       data_at sh_str (tarray tschar (Zlength (sublist (j + 1) (Zlength ls) ls))) 
+               (map Vbyte (sublist (j + 1) (Zlength ls) ls))
+               (Vptr end'_b (Ptrofs.add (Ptrofs.add str_ofs (Ptrofs.repr (j + 1))) Ptrofs.one));
+       data_at sh_end (tptr tschar) (Vptr end'_b end'_ofs) (Vptr end_b end_ofs);
+       data_at sh_intp tlong v (Vptr intp_b intp_ofs))).             
+               (* 0 < s *)
+             easy. 
+               (* s = -1 *)
+             forward.
+             forward.
+             entailer!.
+             (*
+               (Eunop Oneg (Etempvar _value tlong) tlong)
+               going through typechecking functions I found where FF comes from:
+               look at isUnOpResultType or just do Compute below to see it.
+              *)
+             Compute (isUnOpResultType Oneg (Etempvar _value tlong) tlong).
+             (* typecheck error: DEBUG THIS *)
+             admit.
+             entailer.
+             forward.
+             forward.
+             
+             
+             
+             forward_if.
+        
+             3: { 
+
+               (* BREAK: str + j + 1 + 1 >= end *)
+             forward.
+             rewrite_comparison.
+             replace (Ptrofs.unsigned
+          (Ptrofs.add (Ptrofs.add str_ofs (Ptrofs.repr (j + 1)))
+             (Ptrofs.mul (Ptrofs.repr 1) (Ptrofs.of_ints (Int.repr 1)))))
+                     with (Ptrofs.unsigned str_ofs + j + 1 + 1) in *
+               by (autorewrite with norm;
+                   ptrofs_compute_add_mul;
+                   rep_omega_setup;
+                   nia).
+             (* post-if implies break condition *)
+             { Exists j.
+               lt_ub_to_Z H10.
+               lt_ub_to_Z H11.
+               lt_ub_to_Z H12.
+               (* replace Int64 with Int and use vst tactic: *)                   
+               replace (Ptrofs.unsigned str_ofs + j + 1 >=?
+                                                        Ptrofs.unsigned end'_ofs)
+                       with false.
+                entailer!.
+                 repeat split; try easy.
+                 replace (Zlength ls) with (j + 1) by nia.
+                eapply app_is_digit; try easy.
+                replace ls with (sublist 0 (j + 1) ls).
+                erewrite  next_value_lt_ub.
+               (* eapply eq_ub_bounded'_minus;
+                  try eassumption. *)
+                admit.
+                eapply is_digit_to_Z in H9.
+                                          
+                  all: try nia; try
+                eassumption; auto.
+                replace (j + 1) with (Zlength ls) by nia.
+                autorewrite with sublist; auto.
+
+                f_equal.
+                f_equal.
+
+                  replace ls with (sublist 0 (j + 1) ls) at 1.
+                erewrite  next_value_lt_ub.
+                instantiate (1 := (Znth j ls)).
+                unfold Z_of_char.
+                nia.
+                 all: try eassumption; try nia; auto.
+                  replace (j + 1) with (Zlength ls) by nia.
+                autorewrite with sublist; auto.
+              
+               replace (Zlength ls) with (j + 1) by nia; auto. 
+               replace (sublist 1 (j + 1) (i :: ls)) with
+                   (sublist 0 j ls).
+               
+               erewrite sepcon_assoc.
+               replace (Zlength ls - (j + 1))
+                 with (Zlength (sublist (j + 1) (Zlength ls) ls)).
+               erewrite <- DATA_AT1.
+                erewrite sepcon_assoc.
+               erewrite <- DATA_AT2.
+
+           assert (data_at sh_str tschar (Vbyte i) (Vptr end'_b str_ofs) *
+                    data_at sh_str (tarray tschar (Zlength ls)) (map Vbyte ls)
+                       (Vptr end'_b (Ptrofs.add str_ofs Ptrofs.one)) =
+                       data_at sh_str (tarray tschar (Zlength ls + 1)) (Vbyte i :: map Vbyte ls)
+                       (Vptr end'_b str_ofs)) as DATA_AT4.
+           { erewrite <- split_non_empty_list with (ls := i::ls);
+               autorewrite with sublist in H1;
+               autorewrite with sublist;
+               try reflexivity; try nia.
+           }
+               
+           erewrite DATA_AT4.
+           entailer!.
+               all:  try eapply bounded'_bool_to_Prop in H6; auto;
+                 autorewrite with sublist; auto.
+               replace (i :: ls) with (app [i] ls)
+                 by reflexivity.
+               erewrite sublist_app2.
+               all: autorewrite with sublist; try nia; auto.
+               symmetry.
+               rewrite Z.geb_leb.
+               rewrite Z.leb_gt.
+               nia.
+               admit.
+             }
+             } 
+             (* compare pointers *)
+             {  autorewrite with sublist.
+               replace (Zlength (sublist (j + 1) (Zlength ls) ls)) with (Zlength ls - j - 1).
+               
+               unfold test_order_ptrs; simpl.
+               destruct peq; [simpl|contradiction].
+               apply andp_right.
+                destruct (Z_lt_le_dec (j + 1) (Zlength ls)).
+               * apply derives_trans with (Q := valid_pointer
+                                                  (Vptr end'_b
+                                                        (Ptrofs.add
+                                                           (Ptrofs.add
+                                                              str_ofs Ptrofs.one)
+                                                           (Ptrofs.repr (j + 1))))).
+                 entailer!.
+                 replace (Ptrofs.add (Ptrofs.add str_ofs (Ptrofs.repr (j + 1))) Ptrofs.one)
+                   with
+                     (Ptrofs.add (Ptrofs.add str_ofs Ptrofs.one) (Ptrofs.repr (j + 1))).
+                 entailer!.
+                 rewrite Ptrofs.add_assoc.
+                 rewrite Ptrofs.add_assoc.
+                 f_equal.
+                 rewrite Ptrofs.add_commut.
+                 reflexivity.
+                 replace (Ptrofs.add (Ptrofs.add str_ofs Ptrofs.one) (Ptrofs.repr (j + 1)))
+                   with
+                     (Ptrofs.add str_ofs (Ptrofs.repr (j + 1 + 1))).
+                 apply valid_pointer_weak.
+                 replace (Ptrofs.unsigned Ptrofs.one) with 1
+                   by auto with ptrofs.
+                 ptrofs_compute_add_mul;
+                   rep_omega_setup; try nia;
+                      replace (Ptrofs.unsigned Ptrofs.one) with 1
+                   by auto with ptrofs.
+                 f_equal.
+                 all: nia.
+               *  apply derives_trans with (Q := valid_pointer (Vptr end'_b end'_ofs)).
+                 entailer!.
+                 replace end'_ofs with (Ptrofs.add str_ofs (Ptrofs.repr (j + 1 + 1))).
+                 apply valid_pointer_weak.
+                
+                 autorewrite with sublist in LEN.
+                 replace (Zlength ls) with (j + 1) in LEN by nia.
+                 assert (Ptrofs.unsigned str_ofs + j + 1 + 1 = Ptrofs.unsigned end'_ofs)
+                   by nia.
+                 ptrofs_compute_add_mul.
+                 replace end'_ofs with (Ptrofs.repr (Ptrofs.unsigned end'_ofs))
+                   by auto with ints.
+                 f_equal.
+                 all: try (rep_omega_setup; nia).
+               * apply derives_trans with (Q := valid_pointer (Vptr end'_b end'_ofs)).
+                 entailer!.
+                 apply valid_pointer_weak.
+               * erewrite Zlength_sublist.
+                 all: try nia. }
+
+             assert (data_at sh_str tschar (Vbyte i) (Vptr end'_b str_ofs) *
+                          data_at sh_str (tarray tschar (Zlength ls)) (map Vbyte ls)
+                                  (Vptr end'_b (Ptrofs.add str_ofs Ptrofs.one)) =
+                          data_at sh_str (tarray tschar (Zlength ls + 1))
+                                  (Vbyte i :: map Vbyte ls)
+                                  (Vptr end'_b str_ofs)) as DATA_AT4.
+                  { erewrite <- split_non_empty_list with (ls := i::ls);
+                      subst; autorewrite with sublist in H1;
+                      autorewrite with sublist;
+                      try reflexivity; try nia. }
+
+                  
+
+              forward.
+             rewrite_comparison.
+             replace  (Ptrofs.unsigned
+          (Ptrofs.add (Ptrofs.add str_ofs (Ptrofs.repr (j + 1)))
+             (Ptrofs.mul (Ptrofs.repr 1) (Ptrofs.of_ints (Int.repr 1)))))
+                                         with 
+                                           (Ptrofs.unsigned str_ofs + j + 1 + 1) in *
+               by (normalize;ptrofs_compute_add_mul;
+                rep_omega_setup;
+               nia).
+             assert (0 < Zlength (sublist (j + 1) (Zlength ls) ls)).
+
+             { subst.               
+               destruct (Z_lt_le_dec (Ptrofs.unsigned str_ofs + j + 1 + 1) Ptrofs.modulus).                       *
+               erewrite Zlength_sublist.
+               all: try nia.
+               *
+                autorewrite with norm in H11.
+                ptrofs_compute_add_mul.
+                all: try (rep_omega_setup;
+               nia).
+               }
+             edestruct sublist_first with (j := j + 1) (ls := ls) as [i1 Sub2];
+               try nia.
+             econstructor.
+             instantiate (1 := 0); cbv; auto.
+
+            assert (data_at sh_str (tarray tschar (Zlength ls - (j + 1)))
+       (map Vbyte (sublist (j + 1) (Zlength ls) ls))
+       (Vptr end'_b (Ptrofs.add (Ptrofs.add str_ofs (Ptrofs.repr (j + 1))) Ptrofs.one)) =
+        data_at sh_str tschar (Vbyte i1)
+       (Vptr end'_b (Ptrofs.add (Ptrofs.add str_ofs (Ptrofs.repr (j + 1))) Ptrofs.one)) *
+     data_at sh_str (tarray tschar (Zlength (sublist (j + 1 + 1) (Zlength ls) ls)))
+       (map Vbyte (sublist (j + 1 + 1) (Zlength ls) ls))
+       (Vptr end'_b
+          (Ptrofs.add (Ptrofs.add (Ptrofs.add str_ofs (Ptrofs.repr (j + 1))) Ptrofs.one)
+             Ptrofs.one))) as DATA_AT5.
+            {         
+            erewrite Sub2.
+             (* reading a char i1 *)
+            replace (Zlength ls - (j + 1)) with 
+                (Zlength (i1::(sublist (j + 1 + 1) (Zlength ls) ls))).
+            erewrite split_non_empty_list with
+                 (i := i1) (ls' := (sublist (j + 1 + 1) (Zlength ls) ls))
+                 (ofs :=  (Ptrofs.add (Ptrofs.add str_ofs 
+                                                  (Ptrofs.repr (j + 1))) Ptrofs.one));
+             auto.
+            all:      
+              autorewrite with sublist;  
+              ptrofs_compute_add_mul; 
+              replace (Ptrofs.unsigned Ptrofs.one)  with 1 by normalize;
+                try (rep_omega_setup;
+               nia). }
+
+            autorewrite with sublist.
+            erewrite  DATA_AT5.
+              (* str + j + 1 < end *)
+             Intros.
+             forward.
+             forward_if  
+               (temp _t'1 (if 48 <=? Byte.signed i1
+                           then Val.of_bool (Byte.signed i1 <=?  57) 
+                           else Vfalse)).
+             forward.
+             forward.
+             entailer!.
+             
+             { erewrite Z.ge_le_iff in *.
+               erewrite <- Z.leb_le in *.
+               break_if.
+               replace (negb (Int.lt (Int.repr 57) (Int.repr (Byte.signed i1))))
+                 with (Byte.signed i1 <=? 57).
+               destruct (Byte.signed i1 <=? 57); easy.
+               eapply Zge_bool_Intge.
+               easy. }
+             forward.
+             entailer!.
+               { break_if.
+               try rewrite <- Zle_is_le_bool in *.
+               nia.
+               reflexivity. }
+               assert (Znth (j + 1) ls = i1) as ZN1.
+               { replace (i1 :: sublist (j + 1 + 1) (Zlength ls) ls)
+                   with (app [i1] (sublist (j + 1 + 1) (Zlength ls) ls))
+                   in Sub2.
+                 erewrite <- sublist_rejoin' 
+                   with (mid := (j + 1) + 1)
+                        (mid' := (j + 1) + 1)
+                   in Sub2.
+                 eapply app_inv_tail in Sub2.
+                 erewrite  sublist_len_1 in Sub2.
+                 inversion Sub2.
+                 all: auto.
+                 all: try nia.
+               }
+
+               assert ( 0 <= value_until (j + 1) ls) as NN1 by (eapply loop_non_neg; nia).
+               forward_if.
+
+                (* ERROR RANGE spec *)
+               {rewrite <- ZN1 in *.
+                rewrite <- ZN in *.
+                 eapply typed_true_to_digit in H15.
+                 lt_ub_to_Z H10.
+                 lt_ub_to_Z H11.
+                 lt_ub_to_Z H12.
+                 assert ((Byte.signed (Znth j ls) - 48) <= last_digit_max_minus)
+                     by admit. clear H12.
+                 inversion H6.
+                 eapply bounded'_bool_to_Prop in H6.
+
+                 assert (bounded' (value_until (j + 1) ls) = true) as Bound.             
+                  { erewrite next_value_lt_ub with (i := Znth j ls).
+                    admit.
+                    subst; eassumption. 
+                    all: unfold value_until, Z_of_char in *;
+                      subst; try eassumption; try nia; auto.
+                   }
+
+                  assert (bounded' (value_until ((j + 1) + 1) ls) = false) as BoundF.
+             
+                  { 
+                    erewrite next_value_lt_ub with (i := Znth (j + 1) ls).
+                    eapply lt_ub_not_bounded'.
+                    eassumption.
+                    eapply is_digit_to_Z;
+                    eassumption.
+                    erewrite next_value_lt_ub with (i := Znth j ls).
+                    eapply eq_ub_next; try nia
+                     eapply is_digit_to_Z.
+                    all: try eassumption; try nia.
+                    eapply is_digit_to_Z; eassumption; auto.
+                    auto.
+                    eapply app_is_digit; try eassumption; try nia;
+                      auto.
+                    auto. }
+
+                  assert (j + 1 + 1 <= Zlength ls) as LS_len2 by nia.
+
+                  assert (res (Z_of_string_loop' ls 0 1 false) = ERROR_RANGE) as Result_loop.
+                  { 
+                    assert ((Zlength (sublist 0 (j + 1 + 1) ls))
+                            =  (j + 1 + 1)) as SB
+                          by  (erewrite Zlength_sublist;
+                      subst;
+                      try nia).
+                    edestruct all_digits_OK_or_ERROR_RANGE_loop
+                      with (ls := (sublist 0 (j + 1 + 1) ls)) (v:= 0) (i := 1); try rewrite SB.
+                    eapply app_is_digit;  try rewrite SB;
+                    try nia.
+                    eapply app_is_digit;  try rewrite SB;
+                      try nia.                  
+                    intros.
+                    erewrite Znth_sublist.
+                    normalize.
+                    all: try nia.
+                    all: try erewrite Znth_sublist;
+                    try nia; normalize; subst; try eassumption.
+                    eapply OK_bounded'_loop in H12.
+                    congruence.
+                    admit.
+                    eapply sublist_ERROR_RANGE in H12;
+                    subst; try (
+                    eassumption || nia).
+                  }
+
+                  assert (res (Z_of_string (i :: ls)) = ERROR_RANGE) as Result.
+                  {
+                    simpl.
+                    repeat bool_rewrite.
+                    break_match. 
+                    autorewrite with sublist in H2;
+                      try nia.
+                    eassumption.
+                  }                 
+                  assert (index (Z_of_string_loop' ls 0 1 false) = j + 1 + 1) as Index_loop.
+                  { eapply ERROR_RANGE_index; try eassumption;
+                      try nia.
+                  }
+                  assert (index (Z_of_string (i :: ls)) = j + 1 + 1) as Index.
+                  {  simpl.
+                    repeat bool_rewrite.
+                    break_match. 
+                    autorewrite with sublist in H2;
+                      try nia.
+                    eassumption. }                 
+                  forward.
+                  erewrite Result, Index.
+                  entailer!.
+                  autorewrite with sublist in DATA_AT1.
+                  erewrite sepcon_assoc.
+                  erewrite <- DATA_AT5.
+                  erewrite sepcon_assoc.
+                  erewrite <- DATA_AT1.
+                  erewrite sepcon_assoc.
+                  erewrite <- DATA_AT2.
+                  erewrite DATA_AT4.
+                  autorewrite with sublist.
+                   entailer!.
+                   
+                  admit.
+                  admit.
+                  admit.
+                  }
+               forward.
+               forward.
+               entailer!.
+               (* Extra data case *)
+               admit.
+               admit. } 
+             (* end of vl = ub && d <= last_digit *)
+
+             (* vl > ub && d > ld, out of range *)
+             { lt_ub_to_Z H10.
+               eapply lt_ub_to_Z3 in H11.
+               lt_ub_to_Z H12.
+               inversion H6.
+               eapply bounded'_bool_to_Prop in H6.
+              assert (bounded' (value_until (j + 1) ls) = false) as Bound.
+               { erewrite next_value_lt_ub.
+                 eapply  eq_ub_not_bounded'_minus.
+                 eapply loop_non_neg; nia.
+                 eapply is_digit_to_Z; eassumption.
+                 all: unfold value_until, Z_of_char in *;
+                   try eassumption; try nia. } 
+
+               assert (res (Z_of_string_loop' ls 0 1 false) = ERROR_RANGE) as Result_loop.
+               eapply  ub_last_digit_error_range;
+                 try eassumption; try nia.
+
+              assert (res (Z_of_string (i :: ls)) = ERROR_RANGE) as Result.
+               {  simpl.
+                    repeat bool_rewrite.
+                    break_match. 
+                    autorewrite with sublist in H2;
+                      try nia.
+                    eassumption. }  
+
+                 assert (index (Z_of_string_loop' ls 0 1 false) = j + 1 ) as Index_loop.
+                    eapply ERROR_RANGE_index; try eassumption;
+                      try nia.
+
+               assert (index (Z_of_string (i :: ls)) = j + 1) as Index.
+               {  simpl.
+                    repeat bool_rewrite.
+                    break_match. 
+                    autorewrite with sublist in H2;
+                      try nia.
+                    eassumption.                  
+               }                
+               repeat forward.
+               rewrite Result.
+               entailer!.
+               { rewrite Index.             
+                 entailer!.
+                 autorewrite with sublist in DATA_AT1.
+                 erewrite sepcon_assoc.    
+                 autorewrite with sublist.
+                  (erewrite <- DATA_AT1). 
+                   erewrite sepcon_assoc.    
+                   erewrite <- DATA_AT2.
+                  assert (data_at sh_str tschar (Vbyte i) (Vptr end'_b str_ofs) *
+                          data_at sh_str (tarray tschar (Zlength ls)) (map Vbyte ls)
+                                  (Vptr end'_b (Ptrofs.add str_ofs Ptrofs.one)) =
+                          data_at sh_str (tarray tschar (Zlength ls + 1))
+                                  (Vbyte i :: map Vbyte ls)
+                                  (Vptr end'_b str_ofs)) as DATA_AT4.
+                  { erewrite <- split_non_empty_list with (ls := i::ls);
+                      autorewrite with sublist in H1;
+                      autorewrite with sublist;
+                      try reflexivity; try nia. }
+                  erewrite DATA_AT4.
+                 autorewrite with sublist.
+                 entailer!. }
+                all: try  eapply bounded'_bool_to_Prop in H6; 
+                 try nia; try eassumption.
+                 admit. }
+             } (* end of case vl = ub && d > last_digit *)
+             (* case vl > ub *) 
+             { 
+              lt_ub_to_Z H10.
+              eapply lt_ub_to_Z5 in H11.
+              assert (value_until j ls > AbstractSpecLemmas.upper_boundary)
+                     by nia.
+              inversion H6.
+              eapply bounded'_bool_to_Prop in H6.
+
+              assert (bounded' (value_until (j + 1) ls) = false) as Bound.
+                  { erewrite next_value_lt_ub.
+                    eapply lt_ub_not_bounded'.
+                    eapply loop_non_neg; nia.
+                    eapply is_digit_to_Z; eassumption.
+                    all: unfold value_until, Z_of_char in *;
+                      try eassumption; try nia. } 
+
+               assert (res (Z_of_string_loop' ls 0 1 false) = ERROR_RANGE) as Result_loop.
+               eapply  ub_last_digit_error_range;
+                 try eassumption; try nia.
+
+              assert (res (Z_of_string (i :: ls)) = ERROR_RANGE) as Result.
+               {  simpl.
+                    repeat bool_rewrite.
+                    break_match. 
+                    autorewrite with sublist in H2;
+                      try nia.
+                    eassumption.  }  
+
+                 assert (index (Z_of_string_loop' ls 0 1 false) = j + 1 ) as Index_loop.
+                    eapply ERROR_RANGE_index; try eassumption;
+                      try nia.
+
+               assert (index (Z_of_string (i :: ls)) = j + 1) as Index.
+               { simpl.
+                    repeat bool_rewrite.
+                    break_match. 
+                    autorewrite with sublist in H2;
+                      try nia.
+                    eassumption.                  
+               }                
+               repeat forward.
+               rewrite Result.
+               entailer!.
+               { rewrite Index.                
+                 entailer!.
+                 erewrite sepcon_assoc.      
+                 erewrite <- DATA_AT1.
+                 erewrite sepcon_assoc.    
+                 erewrite <- DATA_AT2. 
+                  assert (data_at sh_str tschar (Vbyte i) (Vptr end'_b str_ofs) *
+                          data_at sh_str (tarray tschar (Zlength ls)) (map Vbyte ls)
+                                  (Vptr end'_b (Ptrofs.add str_ofs Ptrofs.one)) =
+                          data_at sh_str (tarray tschar (Zlength ls + 1))
+                                  (Vbyte i :: map Vbyte ls)
+                                  (Vptr end'_b str_ofs)) as DATA_AT4.
+                  { erewrite <- split_non_empty_list with (ls := i::ls);
+                      autorewrite with sublist in H1;
+                      autorewrite with sublist;
+                      try reflexivity; try nia. }
+                  erewrite DATA_AT4.
+                 autorewrite with sublist.
+                 entailer!. }
+               all: try  eapply bounded'_bool_to_Prop in H6; try nia.
+             }
+             (* i0 non-digit: extra data *)
+           { eapply typed_false_to_digit in H9.
+             forward.
+             forward.
+             entailer!.
+             rewrite Int64.signed_repr.
+             eapply bounded'_bool_to_Prop.
+             eapply neg_bounded'; eassumption.
+             eapply bounded'_bool_to_Prop;
+             eassumption.
+             assert ((sublist 0 (j + 1) ls) = 
+                     app (sublist 0 j ls) [i0]) as SL.
+             { erewrite  sublist_split with (mid := j).
+               f_equal.
+               replace (i0 :: sublist (j + 1) (Zlength ls) ls)
+                 with (app [i0] (sublist (j + 1) (Zlength ls) ls))
+                 in Sub.
+               erewrite <- sublist_rejoin' 
+                 with (mid := j + 1)
+                      (mid' := j + 1) in Sub.
+               eapply app_inv_tail in Sub.
+               all: try  eassumption; try nia.
+               reflexivity. }
+
+              assert (res (Z_of_string_loop' (sublist 0 (j + 1) ls) 0 1) = EXTRA_DATA)
+                     as Result_loop_j.
+              { rewrite  SL.
+                eapply EXTRA_DATA_next_loop.
+                eapply  bounded'_to_OK_loop.
+                autorewrite with sublist.
+                eassumption.
+                intros.
+                autorewrite with sublist in H10.
+                replace (Znth i1 (sublist 0 j ls)) with (Znth i1 ls).
+                autorewrite with sublist in H10.
+                eapply H5; try nia; try eassumption.
+                erewrite Znth_sublist.
+                normalize.
+                all: try nia; try eassumption. }
+
+             assert (index (Z_of_string_loop' (sublist 0 (j + 1) ls) 0 1) = j + 1)
+               as Index_loop_j.
+               {
+                 rewrite SL.
+                 replace j with (Zlength (sublist 0 j ls)) at 2
+                                by (autorewrite with sublist; nia).
+                 eapply EXTRA_DATA_index_loop.
+                 eapply  bounded'_to_OK_loop;
+                 autorewrite with sublist; try
+                 eassumption.
+                 intros.
+                 autorewrite with sublist in H10.
+                 replace (Znth i1 (sublist 0 j ls)) with (Znth i1 ls).
+                 autorewrite with sublist in H10.
+                 eapply H5; try nia; try eassumption.
+                 erewrite Znth_sublist.
+                 normalize.
+                 all: try nia; try eassumption.
+               }  
+
+             assert (value (Z_of_string_loop' (sublist 0 (j + 1) ls) 0 1) 
+                     = (value_until false j ls)) as Value_loop_j.
+               {
+                 rewrite SL.
+                 replace j with (Zlength (sublist 0 j ls)) at 2
+                                by (autorewrite with sublist; nia).
+                 autorewrite with sublist.
+                 eapply EXTRA_DATA_value_loop.
+                 eapply  bounded'_to_OK_loop;
+                 autorewrite with sublist; try
+                 eassumption.
+                 intros.
+                 autorewrite with sublist in H10.
+                 replace (Znth i1 (sublist 0 j ls)) with (Znth i1 ls).
+                 autorewrite with sublist in H10.
+                 eapply H5; try nia; try eassumption.
+                 erewrite Znth_sublist.
+                 normalize.
+                 all: try nia; try eassumption.
+               }  
+
+              assert (value (Z_of_string_loop' ls 0 1 false) = value_until j ls) as Value_loop.
+              eapply sublist_EXTRA_DATA  with (j := j + 1) (m := j + 1);
+                try eassumption; auto.
+              
+
+             assert (res (Z_of_string_loop' ls 0 1 false) = EXTRA_DATA) as Result_loop.
+              eapply sublist_EXTRA_DATA  with (j := j + 1) (m := j + 1)
+                                              (vl := value_until (j + 1) ls);
+                try eassumption; auto. 
+
+                assert (index (Z_of_string_loop' ls 0 1 false) = j + 1) as Index_loop.
+              eapply sublist_EXTRA_DATA  with (j := j + 1) (m := j + 1)
+                                              (vl := value_until (j + 1) ls);
+                try eassumption; auto.
+
+
+              assert (index (Z_of_string (i :: ls)) = j + 1) as Index.  
+              { simpl.
+                repeat bool_rewrite.
+                break_match. 
+                autorewrite with sublist in H2;
+                  try nia.
+                eassumption. }
+
+              
+              assert (res (Z_of_string (i :: ls)) = EXTRA_DATA) as Result.           
+              { simpl.
+                repeat bool_rewrite.
+                break_match. 
+                autorewrite with sublist in H2;
+                  try nia.
+                eassumption. }
+               
+             assert ((value (Z_of_string (i :: ls)) =
+               (-1 * value_until j ls)%Z)) as Value.
+               { simpl.
+                 unfold is_sign, minus_char.
+                 bool_rewrite.
+                 break_match.
+                 autorewrite with sublist in *.
+                 nia.
+                 bool_rewrite.
+                 rewrite Value_loop.
+                 reflexivity.
+               }
+             forward.
+             rewrite Result, Index, Value.
+             entailer!.
+             { erewrite sepcon_assoc.      
+               erewrite <- DATA_AT1.
+               erewrite sepcon_assoc.    
+               erewrite <- DATA_AT2.
+               assert (data_at sh_str tschar (Vbyte i) (Vptr end'_b str_ofs) *
+                       data_at sh_str (tarray tschar (Zlength ls)) (map Vbyte ls)
+                               (Vptr end'_b (Ptrofs.add str_ofs Ptrofs.one)) =
+                       data_at sh_str (tarray tschar (Zlength ls + 1))
+                               (Vbyte i :: map Vbyte ls)
+                               (Vptr end'_b str_ofs)) as DATA_AT4.
+               { erewrite <- split_non_empty_list with (ls := i::ls);
+                   autorewrite with sublist in H1;
+                   autorewrite with sublist;
+                   try reflexivity; try nia. }
+               erewrite DATA_AT4.
+                 autorewrite with sublist.
+                 entailer!. }
+               all: try  eapply bounded'_bool_to_Prop in H6; nia.
+             }
+  }   
+        ** admit.
+        ** admit.
+        * reflexivity.
+        * eassumption.
+  - (* str >= end *)
+    all: try apply Z.ltb_ge in IFCON.
+    forward_if.
+    (* Valid pointer proof *)
+    { unfold test_order_ptrs; simpl.
+      destruct peq; [simpl|contradiction].
+      apply andp_right.
+      * apply derives_trans with (Q := valid_pointer (Vptr end'_b str_ofs)).
+        entailer!.
+        apply valid_pointer_weak.
+      * apply derives_trans with (Q := valid_pointer (Vptr end'_b end'_ofs)).
+        entailer!.
+        apply valid_pointer_weak. }
+
+    + (* str >= end, return INVAL *)
+      forward.
+      try apply Z.ltb_ge in IFCON.
+      autorewrite with sublist in *|-.
+      try apply Z.ltb_ge in IFCON.
+      assert ((Ptrofs.unsigned end'_ofs - Ptrofs.unsigned str_ofs) <= 0)
+             by nia.
+      assert (Zlength ls = 0) as L by admit.
+      subst.
+      pose proof Zlength_nil_inv ls L as NIL.
+      rewrite NIL; simpl; entailer!.
+    +  (* end' <= str = true || str < end' = true (from forward_if) *)
+      try apply Z.ltb_lt in IFCON.
+      rewrite EQB in H; apply typed_false_ptr_ge in H.
+      rewrite Z.gtb_lt in H. lia.
+Admitted.
